## 3.2-1

> Show that if $f(n)$ and $g(n)$ are monotonically increasing functions, then so are the functions $f(n) + g(n)$ and $f(g(n))$, and if $f(n)$ and $g(n)$ are in addition nonnegative, then $f(n) \cdot g(n)$ is monotonically increasing.

\begin{align}
f(m) \le f(n) \quad \text{ for } m \le n \\\\
g(m) \le g(n) \quad \text{ for } m \le n, \\\\
\to f(m) + g(m) \le f(n) + g(n),
\end{align}

which proves the first function.

Then

$$f(g(m)) \le f(g(n)) \text{ for } m \le n.$$

This is true, since $g(m) > g(n)$ and $f(n)$ is monotonically increasing.

If both functions are nonnegative, then we can multiply the two equalities and we get

$$f(m) \cdot g(m) \le f(n) \cdot g(n).$$

## 3.2-2

> Prove equation $\text{(3.16)}$.

\begin{align}
a^{\log_b c} = a^\frac{\log_a c}{\log_a b} = (a^{\log_a c})^{\frac{1}{\log_a b}} = c^{\log_b a}
\end{align}

## 3.2-3

> Prove equation $\text{(3.19)}$. Also prove that $n \ne \omega(2^n)$ and $n \ne o(n^n)$.
> 
> $$\lg(n!) = \Theta(n\lg n) \tag{3.19}$$

We use **Stirling's approximation:**

\begin{align}
\lg(n!) 
  & = \lg\Bigg(\sqrt{2\pi n}\Big(\frac{n}{e}\Big)^n\Big(1 + \Theta(\frac{1}{n})\Big)\Bigg) \\\\
  & = \lg\sqrt{2\pi n } + \lg\Big(\frac{n}{e}\Big)^n + \lg\Big(1+\Theta(\frac{1}{n})\Big) \\\\
  & = \Theta(\sqrt n) + n\lg{\frac{n}{e}} + \lg\Big(\Theta(1) + \Theta(\frac{1}{n})\Big) \\\\
  & = \Theta(\sqrt n) + \Theta(n\lg n) + \Theta(\frac{1}{n}) \\\\
  & = \Theta(n\lg n).
\end{align}

The other two are

$$\forall n > 3: 2^n = \underbrace{2 \cdot 2 \cdot \cdots \cdot 2}_\text{n times} < 1 \cdot 2 \cdot \cdots \cdot n = n! \quad \Rightarrow \quad n! = \omega(2^n).$$

and

$$\forall n > 1 : n! = 1 \cdot 2 \cdot \cdots n < \underbrace{n \cdot n \cdot \cdots \cdot n}_\text{n times} = n^n \quad \Rightarrow \quad n! = o(n^n).$$

## 3.2-4 $\star$

> Is the function $\lceil \lg n \rceil!$ polynomially bounded? Is the function $\lceil \lg\lg n \rceil!$ polynomially bounded?

$\lceil \lg n \rceil!$ is not polynomially bounded, but $\lceil \lg\lg n \rceil!$ is.

Proving that a function $f(n)$ is polynomially bounded is equivalent to proving that $\lg(f(n)) = O(\lg n)$ for the following reasons.

- If $f$ is polynomially bounded, then there exist constants $c$, $k$, $n_0$ such that for all $n \ge n_0$, $f(n) \le cn^k$. Hence, $\lg(f(n)) \le kc\lg n$, which, since $c$ and $k$ are constants, means that $\lg(f(n)) = O(\lg n)$.
- Similarly, if $\lg(f(n) = O(\lg n)$, then $f$ is polynomially bounded.

In the following proofs, we will make use of the following two facts:

1. $\lg(n!) = \Theta(n\lg n)$ (by equation $\text{(3.19)}$).
2. $\lceil \lg n \rceil = \Theta(\lg n)$, because
	- $\lceil \lg n \rceil \ge \lg n$
	- $\lceil \lg n \rceil <   \lg n + 1 \le 2\lg n \text{ for all } n \ge 2$

\begin{align}
\lg(\lceil \lg n \rceil!) & = \Theta(\lceil \lg n \rceil \lg \lceil \lg n \rceil) \\\\
                        & = \Theta(\lg n\lg\lg n) \\\\
                        & = \omega(\lg n).
\end{align}

Therefore, $\lg(\lceil \lg n \rceil!) \ne O(\lg n)$, and so $\lceil \lg n \rceil!$ is not polynomially bounded.

\begin{align}
\lg(\lceil \lg\lg n \rceil!) & = \Theta(\lceil \lg\lg n \rceil \lg \lceil \lg\lg n \rceil) \\\\
                             & = \Theta(\lg\lg n\lg\lg\lg n) \\\\
                             & = o((\lg\lg n)^2) \\\\
                             & = o(\lg^2(\lg n)) \\\\
                             & = o(\lg n).
\end{align}

## 3.2-5 $\star$

> Which is asymptotically larger: $\lg(\lg^\*n)$ or $\lg^\*(\lg n)$?

$\lg^\*(\lg n)$ is asymptotically larger because $\lg^\*(\lg n) = \lg^\*n - 1$.

## 3.2-6

> Show that the golden ratio $\phi$ and its conjugate $\hat \phi$ both satisfy the equation $x^2 = x + 1$.

\begin{align}
\phi^2 - \phi - 1
  & = \big(\frac{1 + \sqrt 5}{2}\big)^2 - \frac{1 + \sqrt 5}{2} - 1 \\\\
  & = \frac{1 + 2\sqrt 5 + 5 - 2 - 2\sqrt 5 - 4}{4} \\\\
  & = 0.
\end{align}
\begin{align}
\hat\phi^2 - \hat\phi - 1 
  & = \big(\frac{1 - \sqrt 5}{2}\big)^2 - \frac{1 - \sqrt 5}{2} - 1 \\\\
  & = \frac{1 - 2\sqrt 5 + 5 - 2 + 2\sqrt 5 - 4}{4} \\\\
  & = 0.
\end{align}
  

## 3.2-7

> Prove by induction that the $i$th Fibonacci number satisfies the equality  
>
> $$F_i = \frac{\phi^i - \hat\phi^i}{\sqrt 5},$$
>
> where $\phi$ is the golden ratio and $\hat\phi$ is its conjugate.

We have two base cases: $i = 0$ and $i = 1$. For $i = 0$, we have

\begin{align}
\frac{\phi^0 - \hat\phi^0}{\sqrt 5} 
    & = \frac{1 - 1}{\sqrt 5} \\\\
    & = 0 \\\\
    & = F_0,
\end{align}

and for $i = 1$, we have

\begin{align}
\frac{\phi^1 - \hat\phi^1}{\sqrt 5} 
    & = \frac{(1 + \sqrt 5) - (1 - \sqrt 5)}{2\sqrt 5} \\\\
    & = \frac{2\sqrt 5}{2\sqrt 5} \\\\
    & = 1 \\\\
    & = F_1.
\end{align}

For the inductive case, the inductive hypothesis is that $F_{i - 1} - (\phi^{i - 1} - \hat\phi^{i - 1}) / \sqrt 5$ and $F_{i - 2} = (\phi^{i - 2} - \hat\phi^{i - 2}) / \sqrt 5$. We have

\begin{align}
F_i & = F_{i - 1} + F_{i - 2} & \text{(equation (3.22)} \\\\
    & = \frac{\phi^{i - 1} - \hat\phi^{i - 1}}{\sqrt 5} + \frac{\phi^{i - 2} - \hat\phi^{i - 2}}{\sqrt 5} & \text{(inductive hypothesis)} \\\\
    & = \frac{\phi^{i - 2}(\phi + 1) - \hat\phi^{i - 2}(\hat\phi + 1)}{\sqrt 5}  \\\\
    & = \frac{\phi^{i - 2}\phi^2 - \hat\phi^{i - 2}\hat\phi^2}{\sqrt 5} & \text{(Exercise 3.2-6)} \\\\
    & = \frac{\phi^i - \hat\phi^i}{\sqrt 5}. 
\end{align}

## 3.2-8

> Show that $k\ln k = \Theta(n)$ implies $k = \Theta(n / \ln n)$.

From the symmetry of $\Theta$,

$$k\ln k = \Theta(n) \Rightarrow n = \Theta(k\ln k).$$

Let's find $\ln n$,

$$\ln n = \Theta(\ln(k\ln k)) = \Theta(\ln k + \ln\ln k) = \Theta(\ln k).$$

Let's divide the two,

$$\frac{n}{\ln n} = \frac{\Theta(k\ln k)}{\Theta(\ln k)} = \Theta({\frac{k\ln k}{\ln k}}) = \Theta(k).$$

The last step above follows from the property that any polylogarithmic function grows more slowly than any positive polynomial function, i.e., that for constants $a, b > 0$, we have $\lg^b = o(n^a)$. Substitute $\lg n$ for $n$, $2$ for $b$, and $1$ for $a$, giving $\lg^2(\lg n) = o(\lg n)$.

Therefore, $\lg(\lceil \lg\lg n \rceil!) = O(\lg n)$, and so $\lceil \lg\lg n \rceil!$ is polynomially bounded.
